src/SMT_terms.v
@@ -14,9 +14,10 @@
 (**************************************************************************)
 
 
+Add LoadPath "." as SMTCoq.
 Add LoadPath "bva" as SMTCoq.bva.
 Require Import Bool List Int63 PArray.
-Require Import SMTCoq.Misc SMTCoq.State.
+Require Import Misc State.
 Require Import SMTCoq.bva.BVList.
 
 Local Open Scope array_scope.
@@ -363,7 +364,7 @@ Module Typ.
        symmetry;apply Zeq_is_eq_bool.
        apply Bool.eqb_true_iff.
        apply Peqb_eq.
-         - admit. (* mind the admit here *)
+       apply DTBV.Leq_bv.
       Qed.
 
       Lemma reflect_i_eqb : forall t x y, reflect (x = y) (i_eqb t x y).
